Refactoring splitting `StateSetFormalism.Formula.lean` in separate files

Validator/StateSetFormalism/Formula.lean
@@ -2,6 +2,7 @@ module
 
 public import Mathlib.Data.Set.Operations
 public import Mathlib.Order.Fin.Basic
+public import Validator.StateSetFormalism.PartialModel
 
 /-
 Cannot compile inline/specializing declaration `disjunctionToCNF` as it uses `List.multiply` of
@@ -11,496 +12,17 @@ This limitation may be lifted in the future.
 public import Validator.Basic
 public import Strips.PlanningTask
 
-/-! # Formulas
-This file provides typeclasses for formulas and different operations these formulas can support.
-Note that this file does not implement any of these operations, but it formalizes what these
-operations should do. More specifically the file contains
-* definitions and methods for models, partial models,
-  literals, clauses, cubes, CNF-formulas and DNF-formulas, and
-* type classes for formulas and various operations on formulas.
--/
-
-public section
+namespace Validator
 
 open STRIPS (VarSet)
 
-namespace Validator.Formula
+public section
 
-/-! ## Model -/
-
-/--
-`Model` is usually in the in the context of a formula, where it represents a model of this formula,
-i.e. an assignment of variables making the formula true.
-It is used to show the correctness of operations.
+/-! # Formulas
+This file provides typeclasses for formulas and different operations these formulas can support.
+Note that this file does not implement any of these operations, but it formalizes what these
+operations should do.
 -/
-abbrev Model n := Fin n → Prop
-
-/-- A set of models. -/
-abbrev Models n := Set (Model n)
-
-/-! ## Literal -/
-
-/--
-A Literal is a variable `i` (represented by `(i, true)`) or
-its negation (represented by `(i, false)`).
--/
-@[unbox]
-structure Literal (n : ℕ) where
-  var : Fin n
-  isPos : Bool
-deriving DecidableEq
-
-namespace Literal
-
-def models {n} : Literal n → Models n
-  | ⟨i, true⟩ => { M | M i }
-  | ⟨i, false⟩ => { M | ¬M i }
-
-lemma mem_models {n} (l : Literal n) M : M ∈ l.models ↔ (M l.var ↔ l.isPos) := by
-  simp [models]
-  split
-  all_goals simp
-
-@[expose]
-def negate {n} (l : Literal n) : Literal n :=
-  ⟨l.var, !l.isPos⟩
-
-@[simp]
-lemma models_negate {n} (l : Literal n) : l.negate.models = l.modelsᶜ := by
-  simp only [models, negate]
-  grind only [= Set.mem_compl_iff, usr Set.mem_ofPred_eq]
-
-lemma eq_or_eq_negate_iff_var_eq {n} {l l' : Literal n} :
-    l.var = l'.var ↔ l = l' ∨ l = l'.negate := by
-  rcases l with ⟨v, b⟩
-  rcases l' with ⟨v', b'⟩
-  have := Bool.eq_or_eq_not b b'
-  grind only [negate]
-
-end Literal
-
-/-! ## Clause -/
-
-/-- A clause is a disjuction of literals. -/
-abbrev Clause n := List (Literal n)
-
-namespace Clause
-
-def models {n} (γ : Clause n) : Models n :=
-  { M | ∃ l ∈ γ, M ∈ l.models }
-
-@[simp]
-lemma mem_models {n} (γ : Clause n) M : M ∈ γ.models ↔ ∃ l ∈ γ, M ∈ l.models := by
-  simp [models]
-
-@[simp]
-lemma models_nil {n} : models ([] : Clause n) = ∅ := by
-  simp only [models, List.not_mem_nil, false_and, exists_false, Set.ofPred_false]
-
-@[simp]
-lemma models_append {n} (γ1 γ2 : Clause n) : models (γ1 ++ γ2) = γ1.models ∪ γ2.models := by
-  ext M
-  grind only [models, List.mem_append, Set.mem_ofPred_eq, Set.mem_union]
-
-def vars {n} (γ : Clause n) : VarSet n :=
-  VarSet.ofList (γ.map Literal.var)
-
-@[simp]
-lemma mem_vars {n} (γ : Clause n) {i} : i ∈ γ.vars ↔ ∃ l ∈ γ, l.var = i := by
-  simp only [vars, VarSet.mem_ofList, List.mem_map]
-
-@[simp]
-lemma vars_cons {n} (γ : Clause n) {l} : Clause.vars (l :: γ) = γ.vars.insert l.var := by
-  rw [SetLike.ext_iff]
-  grind only [vars, VarSet.mem_insert, List.map_cons, VarSet.mem_ofList, List.mem_cons]
-
-end Clause
-
-/-! ## Cube -/
-
-/-- A cube is a conjunction of literals. -/
-abbrev Cube n := List (Literal n)
-
-namespace Cube
-
-def models {n} (δ : Cube n) : Models n :=
-  { M | ∀ l ∈ δ, M ∈ l.models }
-
-@[simp]
-lemma mem_models {n} (δ : Cube n) M : M ∈ δ.models ↔ ∀ l ∈ δ, M ∈ l.models := by
-  simp [models]
-
-@[simp]
-lemma models_append {n} (δ1 δ2 : Cube n) : models (δ1 ++ δ2) = δ1.models ∩ δ2.models := by
-  ext M
-  grind only [models, List.mem_append, Set.mem_ofPred_eq, Set.mem_inter_iff]
-
-@[simp]
-lemma models_nil {n} : models ([] : Cube n) = Set.univ := by
-  simp only [models, List.not_mem_nil, IsEmpty.forall_iff, implies_true, Set.ofPred_true]
-
-@[simp]
-lemma models_cons {n l} (δ : Cube n) : models (l :: δ) = l.models ∩ δ.models := by
-  ext M
-  simp only [models, List.mem_cons, forall_eq_or_imp, Set.mem_ofPred_eq, Set.mem_inter_iff]
-
-def vars {n} (δ : Cube n) : VarSet n :=
-  VarSet.ofList (δ.map Literal.var)
-
-@[simp]
-lemma mem_vars {n} (δ : Cube n) i : i ∈ δ.vars ↔ ∃ l ∈ δ, i = l.var := by
-  grind only [vars, Literal, VarSet.mem_ofList, List.mem_map]
-
-@[simp]
-lemma vars_cons {n} (δ : Cube n) {l} : Cube.vars (l :: δ) = δ.vars.insert l.var := by
-  rw [SetLike.ext_iff]
-  grind only [vars, VarSet.mem_insert, List.map_cons, VarSet.mem_ofList, List.mem_cons]
-
--- TODO : remove
-lemma vars_append {n} (δ δ' : Cube n) : Cube.vars (δ ++ δ') = δ.vars ∪ δ'.vars := by
-  rw [SetLike.ext_iff]
-  grind only [vars, VarSet.mem_union, VarSet.mem_ofList, = List.map_append, = List.mem_append]
-
-def consistent {n} (δ : Cube n) : Bool :=
-  δ.all fun l ↦ l.negate ∉ δ
-
-lemma consistent_iff {n} {δ : Cube n} : δ.consistent ↔ δ.models ≠ ∅ := by
-  simp only [consistent, decide_not, List.all_eq_true, Bool.not_eq_eq_eq_not, Bool.not_true,
-    decide_eq_false_iff_not, ne_eq, Set.ext_iff, mem_models, Set.mem_empty_iff_false, iff_false,
-    not_forall, not_exists, not_not, Literal.mem_models]
-  constructor
-  · intro h1
-    use fun i ↦ ⟨i, true⟩ ∈ δ
-    rintro ⟨v, b⟩ h2
-    grind only [Literal.negate]
-  · rintro ⟨M, h1⟩ l h2 h3
-    have h4 := h1 l.negate h3
-    simp only [Literal.negate] at h4
-    grind only
-
-end Cube
-
-/-- The negation of a clause -/
-def Clause.neg {n} (γ : Clause n) : Cube n :=
-  γ.map Literal.negate
-
-lemma Clause.models_neg {n} {γ : Clause n} : γ.neg.models = γ.modelsᶜ := by
-  simp [neg, Cube.models, Clause.models, compl]
-
-/-- The negation of a cube -/
-def Cube.neg {n} (δ : Cube n) : Clause n :=
-  δ.map Literal.negate
-
-lemma Cube.models_neg {n} {δ : Cube n} : δ.neg.models = δ.modelsᶜ := by
-  simp [neg, Cube.models, Clause.models, compl]
-
-/-! ## CNF -/
-
-/-- A CNF-formula is a conjunction of clauses. -/
-abbrev CNF n := List (Clause n)
-
-namespace CNF
-
-def models {n} (φ : CNF n) : Models n :=
-  { M | ∀ γ ∈ φ, M ∈ γ.models }
-
-@[simp]
-lemma mem_models {n} (φ : CNF n) {M} : M ∈ φ.models ↔ ∀ γ ∈ φ, M ∈ γ.models := by
-  simp [models]
-
-@[simp]
-lemma models_nil {n} : CNF.models ([] : CNF n) = Set.univ := by
-  simp only [models, List.not_mem_nil, IsEmpty.forall_iff, implies_true, Set.ofPred_true]
-
-@[simp]
-lemma models_cons {n} (φ : CNF n) {γ} : CNF.models (γ :: φ) = γ.models ∩ φ.models := by
-  simp only [models, List.mem_cons, Clause.models, Set.mem_ofPred_eq, forall_eq_or_imp,
-    Set.inter_def]
-
-@[simp]
-lemma models_append {n} (φ ψ : CNF n) : (φ ++ ψ).models = φ.models ∩ ψ.models := by
-  ext M
-  simp
-  grind
-
-lemma models_mem_empty {n} (φ : CNF n) (h : [] ∈ φ) : φ.models = ∅ := by
-  grind only [mem_models, = Set.mem_empty_iff_false, Clause.mem_models, ← List.not_mem_nil]
-
-def vars {n} (φ : CNF n) : VarSet n :=
-  φ.foldr (fun γ V ↦ V ∪ γ.vars) ∅
-
-@[simp]
-lemma mem_vars {n} (φ : CNF n) {i} : i ∈ φ.vars ↔ ∃ γ ∈ φ, i ∈ γ.vars := by
-  induction φ with
-  | nil => grind only [vars, List.foldr_nil, VarSet.mem_empty, List.not_mem_nil]
-  | cons γ φ ih =>
-    grind only [vars, Clause.mem_vars, List.foldr_cons, VarSet.mem_union, List.mem_cons]
-
-@[simp]
-lemma vars_cons {n γ} {φ : CNF n} : CNF.vars (γ :: φ) = γ.vars ∪ φ.vars := by
-  simp only [SetLike.ext_iff, mem_vars, List.mem_cons, Clause.mem_vars, exists_eq_or_imp,
-    VarSet.mem_union, implies_true]
-
-@[simp]
-lemma forall_iff_subset_models {n} {φ : CNF n} {Ms} : (∀ γ ∈ φ, Ms ⊆ γ.models) ↔ Ms ⊆ φ.models := by
-  grind only [Set.subset_def, Clause.mem_models, models, Set.mem_ofPred_eq]
-
-lemma models_equiv_right {n} {φ : CNF n} {M M' : Formula.Model n} :
-    (∀ i ∈ vars φ, M i = M' i) → M ∈ models φ → M' ∈ models φ := by
-  simp [Literal.mem_models]
-  grind
-
-end CNF
-
-/-! ## DNF -/
-
-/-- A DNF-formula is a conjunction of cubes. -/
-abbrev DNF n := List (Cube n)
-
-def DNF.models {n} (φ : DNF n) : Models n :=
-  { M |  ∃ δ ∈ φ, M ∈ δ.models }
-
-@[simp]
-lemma DNF.mem_models {n} (φ : DNF n) {M} : M ∈ φ.models ↔ ∃ δ ∈ φ, M ∈ δ.models := by
-  simp [models]
-
-@[simp]
-lemma DNF.exists_iff_models_subset {n} {φ : DNF n} {Ms} :
-    (∀ δ ∈ φ, δ.models ⊆ Ms) ↔ φ.models ⊆ Ms := by
-  grind only [Set.subset_def, Cube.mem_models, models, Set.mem_ofPred_eq]
-
-/-! ## PartialModel -/
-/-- Partial models are partial assignments. In contrast to `Model`, these are used at runtime. -/
-structure PartialModel (n : ℕ) where
-  pos : VarSet n
-  neg : VarSet n
-  disjoint : pos ∩ neg = ∅
-  deriving DecidableEq
-
-namespace PartialModel
-
-@[simps]
-instance {n} : Membership (Literal n) (PartialModel n) where
-  mem M
-  | ⟨i, true⟩ => i ∈ M.pos
-  | ⟨i, false⟩ => i ∈ M.neg
-
-lemma mem_iff {n} (M : PartialModel n) l :
-    l ∈ M ↔ l.var ∈ M.pos ∧ l.isPos ∨ l.var ∈ M.neg ∧ ¬l.isPos := by
-  rw [mem_def]
-  grind only
-
-instance {n l} {M : PartialModel n} : Decidable (l ∈ M) := by
-  rw [mem_def]
-  split
-  all_goals
-    exact VarSet.instDecidableMemFin
-
-def vars {n} (M : PartialModel n) : VarSet n :=
-  M.pos ∪ M.neg
-
-lemma vars_eq {n} (M : PartialModel n) : M.vars = M.pos ∪ M.neg := (rfl)
-
-lemma mem_vars {n i} {M : PartialModel n} : i ∈ M.vars ↔ ∃ l ∈ M, l.var = i := by
-  simp only [vars_eq, VarSet.mem_union, mem_iff]
-  constructor
-  · rintro (h | h)
-    · use ⟨i, true⟩; grind only
-    · use ⟨i, false⟩; grind only
-  · grind only
-
-/-- All models corresponding to to partial model `M`. -/
-def models {n} (M : PartialModel n) : Models n :=
-  { M' | (∀ i ∈ M.pos, M' i) ∧ (∀ i ∈ M.neg, ¬ M' i) }
-
-lemma mem_models' {n} (M : PartialModel n) {M'} :
-    M' ∈ M.models ↔ (∀ i ∈ M.pos, M' i) ∧ (∀ i ∈ M.neg, ¬ M' i) := by
-  simp [models]
-
-lemma mem_models {n} {M : PartialModel n} {M'} : M' ∈ M.models ↔ ∀ l ∈ M, M' ∈ l.models := by
-  simp only [models, Set.mem_ofPred_eq, Literal.models]
-  constructor
-  · grind [mem_def]
-  · intro h1
-    constructor
-    · intro i hi
-      specialize h1 ⟨i, true⟩ hi
-      simp_all only [Set.mem_ofPred_eq]
-    · intro i hi
-      specialize h1 ⟨i, false⟩ hi
-      simp_all only [Set.mem_ofPred_eq, not_false_eq_true]
-
-lemma models_nonempty {n} (M : PartialModel n) : M.models.Nonempty := by
-  use fun i ↦ ⟨i, true⟩ ∈ M
-  simp only [mem_models, Literal.mem_models, mem_def]
-  intro l
-  split
-  case h_1 l i => tauto
-  case h_2 l i =>
-    have := M.disjoint
-    simp_all only [SetLike.ext_iff, VarSet.mem_inter, VarSet.mem_empty, iff_false, not_and,
-      Bool.false_eq_true]
-    grind only [mem_def]
-
--- TODO : remove?
-lemma subset_models_of_mem {n} {M : PartialModel n} {l} : l ∈ M →  M.models ⊆ l.models := by
-  simp [Set.subset_def, mem_models]
-  grind
-
-def empty {n} : PartialModel n :=
-  ⟨∅, ∅, by simp⟩
-
-@[simp]
-lemma vars_empty {n} : (@empty n).vars = ∅ := by
-  simp only [empty, vars_eq, VarSet.union_empty]
-
-@[simp]
-lemma models_empty {n} : (@empty n).models = Set.univ := by
-  simp [empty, Set.ext_iff, mem_models]
-  grind
-
-/-- Returns none if the negation of the literal already occurs in M -/
-def insert {n} (M : PartialModel n) : Literal n → Option (PartialModel n)
-  | ⟨i, true⟩ =>
-    if h : i ∈ M.neg then
-      none
-    else
-      some { M with
-        pos := M.pos.insert i
-        disjoint := by
-          have := M.disjoint
-          grind only [VarSet.inter_eq_empty_iff, VarSet.mem_insert]
-        }
-  | ⟨i, false⟩ =>
-    if h : i ∈ M.pos then
-      none
-    else
-      some { M with
-        neg := M.neg.insert i
-        disjoint := by
-          have := M.disjoint
-          grind only [VarSet.inter_eq_empty_iff, VarSet.mem_insert]
-        }
-
-@[simp]
-lemma insert_eq_none_iff {n} {M : PartialModel n} {l} : M.insert l = none ↔ l.negate ∈ M := by
-  simp [mem_def, insert, Literal.negate]
-  grind
-
-@[simp]
-lemma insert_eq_some_iff {n} {M M' : PartialModel n} {l} :
-    M.insert l = some M' ↔ l.negate ∉ M ∧ ∀ l', l' ∈ M' ↔ l' ∈ M ∨ l' = l := by
-  simp only [insert, mem_def, Literal.negate]
-  split
-  all_goals
-    simp only [Option.dite_none_left_eq_some, Option.some.injEq]
-    constructor
-    · grind only [VarSet.mem_insert]
-    · rintro ⟨h1, h2⟩
-      use h1
-      congr 1
-      all_goals
-        simp only [SetLike.ext_iff, VarSet.mem_insert]
-        intro i
-        have h3 := h2 ⟨i, false⟩
-        specialize h2 ⟨i, true⟩
-        grind only
-
-lemma vars_insert {n} {M M' : PartialModel n} {l} (h : M.insert l = some M') :
-    M'.vars = M.vars.insert l.var := by
-  have ⟨h1, h2⟩ := insert_eq_some_iff.1 h
-  simp only [SetLike.ext_iff, mem_vars, h2, VarSet.mem_insert]
-  grind
-
-lemma models_insert {n} {M M' : PartialModel n} {l} :
-    M.insert l = some M' → M'.models = M.models ∩ l.models := by
-  simp only [insert_eq_some_iff, Set.ext_iff, mem_models, Set.mem_inter_iff]
-  grind
-
-def foldl {α n} (f : α → Literal n → α) (init : α) (M : PartialModel n) : α :=
-  M.pos.foldl (fun a i ↦ f a ⟨i, true⟩) (M.neg.foldl (fun a i ↦ f a ⟨i, false⟩) init)
-
-lemma foldl_cons {α n} {M : PartialModel n} {f : Literal n → α} {a} :
-    a ∈ M.foldl (fun a l ↦ f l :: a) [] ↔ ∃ l ∈ M, a = f l := by
-  simp only [foldl, VarSet.foldl_cons, List.not_mem_nil, or_false, mem_def]
-  grind
-
-def toCNF {n} (M : PartialModel n) : CNF n :=
-  M.foldl (fun φ l ↦ [l] :: φ) []
-
-lemma mem_toCNF {n} {M : PartialModel n} {γ} : γ ∈ M.toCNF ↔ ∃ l ∈ M, γ = [l] := by
-  simp [toCNF, foldl_cons, mem_def]
-
-lemma models_toCNF {n} {M : PartialModel n} : M.toCNF.models = M.models := by
-  ext M'
-  simp only [CNF.mem_models, mem_toCNF, Clause.mem_models, forall_exists_index, and_imp,
-    mem_models]
-  grind only [= List.mem_cons, ← List.not_mem_nil]
-
-def toCube {n} (M : PartialModel n) : Cube n :=
-  M.foldl (fun δ l ↦ l :: δ) []
-
-@[simp]
-lemma vars_toCube {n} {M : PartialModel n} : M.toCube.vars = M.vars := by
-  simp [toCube, foldl_cons, mem_vars, SetLike.ext_iff, Cube.mem_vars]
-  grind only
-
-@[simp]
-lemma models_toCube {n} {M : PartialModel n} : M.toCube.models = M.models := by
-  ext M'
-  simp [toCube, foldl_cons, mem_models]
-
-end PartialModel
-
-namespace Cube
-/-- Translate `δ` to a partial model. Returns `none` if `δ` is inconsistent. -/
-def toPartialModel {n} (δ : Cube n) : Option (PartialModel n) :=
-  δ.foldlM PartialModel.insert PartialModel.empty
-
-@[simp]
-lemma toPartialModel_eq_none_iff {n} {δ : Cube n} :
-    δ.toPartialModel = none ↔ δ.models = ∅ := by
-  suffices h1 : ∀ M, δ.foldlM PartialModel.insert M = none ↔ δ.models ∩ M.models = ∅ by
-    have := h1 PartialModel.empty
-    simp_all only [PartialModel.models_empty, Set.inter_univ, toPartialModel]
-  induction δ with
-  | nil =>
-    intro M
-    have := M.models_nonempty
-    simp_all only [List.foldlM_nil, Option.pure_def, reduceCtorEq, models, List.not_mem_nil,
-      IsEmpty.forall_iff, implies_true, Set.ofPred_true, Set.univ_inter, Set.nonempty_iff_ne_empty]
-  | cons l δ' ih =>
-    intro M
-    simp only [List.foldlM_cons, Option.bind_eq_bind, Option.bind_eq_none_iff, models_cons, ih]
-    cases h1 : M.insert l with
-    | none =>
-      simp only [reduceCtorEq, IsEmpty.forall_iff, implies_true, Set.inter_assoc, true_iff]
-      rw [PartialModel.insert_eq_none_iff] at h1
-      apply PartialModel.subset_models_of_mem at h1
-      grind [Literal.models_negate]
-    | some M' =>
-      have := M.models_insert h1
-      grind only [PartialModel.insert_eq_some_iff, Option.some.injEq]
-
-@[simp]
-lemma models_toPartialModel {n} {δ : Cube n} {M} :
-    δ.toPartialModel = some M → M.models = δ.models := by
-  suffices h1 :
-    ∀ M', (δ.foldlM PartialModel.insert M') = some M → M.models = δ.models ∩ M'.models by
-    intro h2
-    have := h1 PartialModel.empty h2
-    simp_all only [PartialModel.models_empty, Set.inter_univ]
-  induction δ generalizing M with
-  | nil =>
-    grind only [models, = List.foldlM_nil, = Option.pure_apply, = Set.mem_inter_iff,
-      usr Set.mem_ofPred_eq, ← List.not_mem_nil]
-  | cons l δ' ih =>
-    simp_all only [List.foldlM_cons, Option.bind_eq_bind, models_cons, Option.bind_eq_some_iff]
-    rintro M'' ⟨M', h3, h4⟩
-    grind only [PartialModel.models_insert h3]
-
-end Formula.Cube
-
 
 /-! ## Formula -/
 
@@ -513,28 +35,126 @@ class Formula n (R : Type) where
   vars : (φ : R) → VarSet n
 
   /-- The models of the formula `φ` -/
-  models : (φ : R) → Formula.Models n
+  models : (φ : R) → Models n
 
   /--
   If two assignments coincide on the variables of `φ`, then the second is a model of `φ`
   if the first one is a model of `φ`.
   -/
-  models_equiv_right (φ : R) (M M' : Formula.Model n) :
+  models_equiv_right (φ : R) (M M' : Model n) :
     (∀ i ∈ vars φ, M i = M' i) → M ∈ models φ → M' ∈ models φ
-
-namespace Formula
 
 /--
 If two assignments `M` and `M'` coincide on the variables of `φ`, then `M` is a model of
 `φ` iff `M'` is a model of `φ`.
 -/
-lemma models_equiv {n} {R} [h : Formula n R] {φ : R} {M M' : Model n}
+lemma Formula.models_equiv {n} {R} [h : Formula n R] {φ : R} {M M' : Model n}
     (h1 : ∀ i ∈ h.vars φ, M i = M' i) : M ∈ h.models φ ↔ M' ∈ h.models φ := by
   constructor
   · apply models_equiv_right
     exact h1
   · apply models_equiv_right
     grind
+
+/-! ## Renaming -/
+
+structure Renaming {n} (dom : VarSet n) where
+  rename : Fin n → Fin n
+  mono : StrictMonoOn rename dom
+  --prop : ∀ i ∉ dom.toVarSet, rename i = i
+
+lemma Renaming.ne {n} {dom : VarSet n} {r : Renaming dom} :
+    ∀ i ∈ dom, ∀ j ∈ dom, i ≠ j → r.rename i ≠ r.rename j := by
+  intro i hi j hj
+  exact Set.InjOn.ne (StrictMonoOn.injOn r.mono) hi hj
+
+-- TODO : the name is a bit misleading, since it does the inverse of the other rename functions
+@[expose]
+def Model.rename {n} {dom : VarSet n} (r : Renaming dom) (M : Model n) : Model n :=
+  fun i ↦ M (r.rename i)
+
+@[expose]
+def Literal.rename {n} {dom : VarSet n} (r : Renaming dom) (l : Literal n) : Literal n :=
+  ⟨r.rename l.var, l.isPos⟩
+
+@[simp]
+lemma Literal.models_rename {n dom} {r : Renaming dom} {l : Literal n} :
+    (l.rename r).models = Model.rename r ⁻¹' l.models := by
+  ext M
+  simp only [rename, mem_models, Set.mem_preimage, Model.rename]
+
+@[expose]
+def Clause.rename {n} {dom : VarSet n} (r : Renaming dom) (γ : Clause n) : Clause n :=
+  γ.map (Literal.rename r)
+
+@[simp]
+lemma Clause.models_rename {n dom} {r : Renaming dom} {γ : Clause n} :
+    (γ.rename r).models = Model.rename r ⁻¹' γ.models := by
+  ext M
+  simp only [rename, mem_models, List.mem_map, exists_exists_and_eq_and, Literal.models_rename,
+    Set.mem_preimage]
+
+def Cube.rename {n} {dom : VarSet n} (r : Renaming dom) (δ : Cube n) : Cube n :=
+  δ.map (Literal.rename r)
+
+@[expose]
+def CNF.rename {n} {dom : VarSet n} (r : Renaming dom) (φ : CNF n) : CNF n :=
+  φ.map (Clause.rename r)
+
+@[simp]
+lemma CNF.mem_vars_rename {n} {dom : VarSet n} {r : Renaming dom} {φ : CNF n} {i} :
+    i ∈ (φ.rename r).vars ↔ ∃ j ∈ φ.vars, i = r.rename j := by
+  simp [rename, mem_vars, List.mem_map, Clause.rename, Clause.mem_vars,
+    exists_exists_and_eq_and, Literal.rename, ↓existsAndEq, and_true]
+  grind only
+
+@[simp]
+lemma CNF.models_rename {n} {dom : VarSet n} {r : Renaming dom} {φ : CNF n} :
+    (φ.rename r).models = Model.rename r ⁻¹' φ.models := by
+  ext M
+  simp only [mem_models, Set.mem_preimage]
+  simp only [rename, List.mem_map, forall_exists_index, and_imp, forall_apply_eq_imp_iff₂]
+  simp only [Clause.models_rename, Set.mem_preimage]
+
+def VarSet.rename {n} {dom : VarSet n} (r : Renaming dom) (V : VarSet n) : VarSet n :=
+  V.map r.rename
+
+@[simp]
+lemma VarSet.mem_rename {n} {dom : VarSet n} {r : Renaming dom} {V : VarSet n} {i} :
+    i ∈ (VarSet.rename r V) ↔ ∃ j ∈ V, i = r.rename j := by
+  simp [rename, VarSet.mem_map]
+
+def PartialModel.rename {n} {dom : VarSet n} (r : Renaming dom) (M : PartialModel n)
+    (h1 : M.vars ⊆ dom) : PartialModel n where
+  pos := VarSet.rename r M.pos
+  neg := VarSet.rename r M.neg
+  disjoint := by
+    have h3 := r.mono
+    simp only [VarSet.inter_eq_empty_iff, VarSet.mem_rename, not_exists, not_and,
+      forall_exists_index, and_imp]
+    intro _ i hi rfl j hj
+    apply Renaming.ne
+    · apply h1
+      simp [PartialModel.vars_eq, hi]
+    · apply h1
+      simp [PartialModel.vars_eq, hj]
+    · have h2 := M.disjoint
+      grind only [VarSet.inter_eq_empty_iff]
+
+@[simp]
+lemma PartialModel.mem_vars_rename {n dom} {r : Renaming dom} {M : PartialModel n} {h1 i} :
+    i ∈ (M.rename r h1).vars ↔ ∃ j ∈ M.vars, i = r.rename j := by
+  grind only [rename, vars_eq, VarSet.mem_union, VarSet.mem_rename]
+
+@[simp]
+lemma PartialModel.models_rename {n dom} {r : Renaming dom} {M : PartialModel n} {h1} :
+    (M.rename r h1).models = M.models.preimage (Model.rename r) := by
+  ext M'
+  simp only [rename, mem_models', VarSet.mem_rename, forall_exists_index, and_imp, Set.mem_preimage,
+    Model.rename]
+  grind
+
+namespace Formula
 
 /-! ## Operations on Formulas -/
 -- TODO : documentation
@@ -644,88 +264,6 @@ class OfPartialModel n R [F : Formula n R] where
 
   models_ofPartialModel M : F.models (ofPartialModel M) = M.models
 
-structure Renaming {n} (dom : VarSet n) where
-  rename : Fin n → Fin n
-  mono : StrictMonoOn rename dom
-  --prop : ∀ i ∉ dom.toVarSet, rename i = i
-
-lemma Renaming.ne {n} {dom : VarSet n} {r : Renaming dom} :
-    ∀ i ∈ dom, ∀ j ∈ dom, i ≠ j → r.rename i ≠ r.rename j := by
-  intro i hi j hj
-  exact Set.InjOn.ne (StrictMonoOn.injOn r.mono) hi hj
-
--- TODO : the name is a bit misleading, since it does the inverse of the other rename functions
-@[expose]
-def Model.rename {n} {dom : VarSet n} (r : Renaming dom) (M : Model n) : Model n :=
-  fun i ↦ M (r.rename i)
-
-@[expose]
-def Literal.rename {n} {dom : VarSet n} (r : Renaming dom) (l : Literal n) : Literal n :=
-  ⟨r.rename l.var, l.isPos⟩
-
-@[expose]
-def Clause.rename {n} {dom : VarSet n} (r : Renaming dom) (γ : Clause n) : Clause n :=
-  γ.map (Literal.rename r)
-
-def Cube.rename {n} {dom : VarSet n} (r : Renaming dom) (δ : Cube n) : Cube n :=
-  δ.map (Literal.rename r)
-
-@[expose]
-def CNF.rename {n} {dom : VarSet n} (r : Renaming dom) (φ : CNF n) : CNF n :=
-  φ.map (Clause.rename r)
-
-@[simp]
-lemma CNF.mem_vars_rename {n} {dom : VarSet n} {r : Renaming dom} {φ : CNF n} {i} :
-    i ∈ (φ.rename r).vars ↔ ∃ j ∈ φ.vars, i = r.rename j := by
-  simp [rename, mem_vars, List.mem_map, Clause.rename, Clause.mem_vars,
-    exists_exists_and_eq_and, Literal.rename, ↓existsAndEq, and_true]
-  grind only
-
-@[simp]
-lemma CNF.models_rename {n} {dom : VarSet n} {r : Renaming dom} {φ : CNF n} :
-    (φ.rename r).models = φ.models.preimage (Model.rename r) := by
-  simp only [models, rename, List.mem_map, Clause.rename, Clause.models, Literal.mem_models,
-    Set.mem_ofPred_eq, forall_exists_index, and_imp, forall_apply_eq_imp_iff₂, Literal.rename,
-    exists_exists_and_eq_and, Set.preimage_ofPred_eq, Model.rename]
-
-def VarSet.rename {n} {dom : VarSet n} (r : Renaming dom) (V : VarSet n) : VarSet n :=
-  V.map r.rename
-
-@[simp]
-lemma VarSet.mem_rename {n} {dom : VarSet n} {r : Renaming dom} {V : VarSet n} {i} :
-    i ∈ (VarSet.rename r V) ↔ ∃ j ∈ V, i = r.rename j := by
-  simp [rename, VarSet.mem_map]
-
-def PartialModel.rename {n} {dom : VarSet n} (r : Renaming dom) (M : PartialModel n)
-    (h1 : M.vars ⊆ dom) : PartialModel n where
-  pos := VarSet.rename r M.pos
-  neg := VarSet.rename r M.neg
-  disjoint := by
-    have h3 := r.mono
-    simp only [VarSet.inter_eq_empty_iff, VarSet.mem_rename, not_exists, not_and,
-      forall_exists_index, and_imp]
-    intro _ i hi rfl j hj
-    apply Renaming.ne
-    · apply h1
-      simp [PartialModel.vars, hi]
-    · apply h1
-      simp [PartialModel.vars, hj]
-    · have h2 := M.disjoint
-      grind only [VarSet.inter_eq_empty_iff]
-
-@[simp]
-lemma PartialModel.mem_vars_rename {n dom} {r : Renaming dom} {M : PartialModel n} {h1 i} :
-    i ∈ (M.rename r h1).vars ↔ ∃ j ∈ M.vars, i = r.rename j := by
-  grind only [rename, vars_eq, VarSet.mem_union, VarSet.mem_rename]
-
-@[simp]
-lemma PartialModel.models_rename {n dom} {r : Renaming dom} {M : PartialModel n} {h1} :
-    (M.rename r h1).models = M.models.preimage (Model.rename r) := by
-  ext M'
-  simp only [models, rename, VarSet.mem_rename, forall_exists_index, and_imp, Set.mem_ofPred_eq,
-    Set.preimage_ofPred_eq, Model.rename]
-  grind
-
 /-- Renaming consistent with order -/
 class Rename n R [F : Formula n R] where
   --rename (φ : R) (r : { i : Fin n // i ∈ (F.vars φ).val } → Fin n) (h : StrictMono r) : R
@@ -812,5 +350,3 @@ lemma models_negToCNF {n} {R} [F : Formula n R] [h : ToDNF n R] {φ} :
   simp only [negToCNF, CNF.mem_models, List.mem_map, forall_exists_index, and_imp,
     ← models_toDNF]
   grind only [Set.mem_compl_iff, DNF.mem_models, !Cube.models_neg]
-
-end Validator.Formula.ToDNF
