Validator/StateSetFormalism/PartialModel.lean
@@ -1,0 +1,241 @@
+module
+
+public import Validator.StateSetFormalism.Basic
+
+/-! # PartialModel
+This file provides the definition of partial models and operations and lemmas for working with them.
+-/
+
+namespace Validator
+
+open STRIPS (VarSet)
+
+public section
+
+/-- Partial models are partial assignments. In contrast to `Model`, these are used at runtime. -/
+structure PartialModel (n : ℕ) where
+  pos : VarSet n
+  neg : VarSet n
+  disjoint : pos ∩ neg = ∅
+deriving DecidableEq
+
+namespace PartialModel
+
+@[simps]
+instance {n} : Membership (Literal n) (PartialModel n) where
+  mem M
+  | ⟨i, true⟩ => i ∈ M.pos
+  | ⟨i, false⟩ => i ∈ M.neg
+
+lemma mem_iff {n} (M : PartialModel n) l :
+    l ∈ M ↔ l.var ∈ M.pos ∧ l.isPos ∨ l.var ∈ M.neg ∧ ¬l.isPos := by
+  rw [mem_def]
+  grind only
+
+instance {n l} {M : PartialModel n} : Decidable (l ∈ M) := by
+  rw [mem_def]
+  split
+  all_goals
+    exact VarSet.instDecidableMemFin
+
+def vars {n} (M : PartialModel n) : VarSet n :=
+  M.pos ∪ M.neg
+
+lemma vars_eq {n} (M : PartialModel n) : M.vars = M.pos ∪ M.neg := (rfl)
+
+lemma mem_vars {n i} {M : PartialModel n} : i ∈ M.vars ↔ ∃ l ∈ M, l.var = i := by
+  simp only [vars_eq, VarSet.mem_union, mem_iff]
+  constructor
+  · rintro (h | h)
+    · use ⟨i, true⟩; grind only
+    · use ⟨i, false⟩; grind only
+  · grind only
+
+/-- All models corresponding to to partial model `M`. -/
+def models {n} (M : PartialModel n) : Models n :=
+  { M' | (∀ i ∈ M.pos, M' i) ∧ (∀ i ∈ M.neg, ¬ M' i) }
+
+lemma mem_models' {n} (M : PartialModel n) {M'} :
+    M' ∈ M.models ↔ (∀ i ∈ M.pos, M' i) ∧ (∀ i ∈ M.neg, ¬ M' i) := by
+  simp [models]
+
+lemma mem_models {n} {M : PartialModel n} {M'} : M' ∈ M.models ↔ ∀ l ∈ M, M' ∈ l.models := by
+  simp only [models, Set.mem_ofPred_eq, Literal.mem_models]
+  constructor
+  · grind [mem_def]
+  · intro h1
+    constructor
+    · intro i hi
+      specialize h1 ⟨i, true⟩ hi
+      grind only
+    · intro i hi
+      specialize h1 ⟨i, false⟩ hi
+      grind only
+
+lemma models_nonempty {n} (M : PartialModel n) : M.models.Nonempty := by
+  use fun i ↦ ⟨i, true⟩ ∈ M
+  simp only [mem_models, Literal.mem_models, mem_def]
+  intro l
+  split
+  case h_1 l i => simp only [iff_true, imp_self]
+  case h_2 l i =>
+    have := M.disjoint
+    simp_all only [SetLike.ext_iff, VarSet.mem_inter, VarSet.mem_empty, iff_false, not_and,
+      Bool.false_eq_true]
+    grind only [mem_def]
+
+-- TODO : remove?
+lemma subset_models_of_mem {n} {M : PartialModel n} {l} : l ∈ M →  M.models ⊆ l.models := by
+  simp [Set.subset_def, mem_models]
+  grind
+
+def empty {n} : PartialModel n :=
+  ⟨∅, ∅, by simp⟩
+
+@[simp]
+lemma vars_empty {n} : (@empty n).vars = ∅ := by
+  simp only [empty, vars_eq, VarSet.union_empty]
+
+@[simp]
+lemma models_empty {n} : (@empty n).models = Set.univ := by
+  simp [empty, Set.ext_iff, mem_models]
+  grind
+
+/-- Returns none if the negation of the literal already occurs in M -/
+def insert {n} (M : PartialModel n) : Literal n → Option (PartialModel n)
+  | ⟨i, true⟩ =>
+    if h : i ∈ M.neg then
+      none
+    else
+      some { M with
+        pos := M.pos.insert i
+        disjoint := by
+          have := M.disjoint
+          grind only [VarSet.inter_eq_empty_iff, VarSet.mem_insert]
+        }
+  | ⟨i, false⟩ =>
+    if h : i ∈ M.pos then
+      none
+    else
+      some { M with
+        neg := M.neg.insert i
+        disjoint := by
+          have := M.disjoint
+          grind only [VarSet.inter_eq_empty_iff, VarSet.mem_insert]
+        }
+
+@[simp]
+lemma insert_eq_none_iff {n} {M : PartialModel n} {l} : M.insert l = none ↔ l.negate ∈ M := by
+  simp [mem_def, insert, Literal.negate]
+  grind
+
+@[simp]
+lemma insert_eq_some_iff {n} {M M' : PartialModel n} {l} :
+    M.insert l = some M' ↔ l.negate ∉ M ∧ ∀ l', l' ∈ M' ↔ l' ∈ M ∨ l' = l := by
+  simp only [insert, mem_def, Literal.negate]
+  split
+  all_goals
+    simp only [Option.dite_none_left_eq_some, Option.some.injEq]
+    constructor
+    · grind only [VarSet.mem_insert]
+    · rintro ⟨h1, h2⟩
+      use h1
+      congr 1
+      all_goals
+        simp only [SetLike.ext_iff, VarSet.mem_insert]
+        intro i
+        have h3 := h2 ⟨i, false⟩
+        specialize h2 ⟨i, true⟩
+        grind only
+
+lemma vars_insert {n} {M M' : PartialModel n} {l} (h : M.insert l = some M') :
+    M'.vars = M.vars.insert l.var := by
+  have ⟨h1, h2⟩ := insert_eq_some_iff.1 h
+  simp only [SetLike.ext_iff, mem_vars, h2, VarSet.mem_insert]
+  grind
+
+lemma models_insert {n} {M M' : PartialModel n} {l} :
+    M.insert l = some M' → M'.models = M.models ∩ l.models := by
+  simp only [insert_eq_some_iff, Set.ext_iff, mem_models, Set.mem_inter_iff]
+  grind
+
+def foldl {α n} (f : α → Literal n → α) (init : α) (M : PartialModel n) : α :=
+  M.pos.foldl (fun a i ↦ f a ⟨i, true⟩) (M.neg.foldl (fun a i ↦ f a ⟨i, false⟩) init)
+
+lemma foldl_cons {α n} {M : PartialModel n} {f : Literal n → α} {a} :
+    a ∈ M.foldl (fun a l ↦ f l :: a) [] ↔ ∃ l ∈ M, a = f l := by
+  simp only [foldl, VarSet.foldl_cons, List.not_mem_nil, or_false, mem_def]
+  grind
+
+def toCNF {n} (M : PartialModel n) : CNF n :=
+  M.foldl (fun φ l ↦ [l] :: φ) []
+
+lemma mem_toCNF {n} {M : PartialModel n} {γ} : γ ∈ M.toCNF ↔ ∃ l ∈ M, γ = [l] := by
+  simp [toCNF, foldl_cons, mem_def]
+
+lemma models_toCNF {n} {M : PartialModel n} : M.toCNF.models = M.models := by
+  ext M'
+  simp only [CNF.mem_models, mem_toCNF, Clause.mem_models, forall_exists_index, and_imp,
+    mem_models]
+  grind only [= List.mem_cons, ← List.not_mem_nil]
+
+def toCube {n} (M : PartialModel n) : Cube n :=
+  M.foldl (fun δ l ↦ l :: δ) []
+
+@[simp]
+lemma vars_toCube {n} {M : PartialModel n} : M.toCube.vars = M.vars := by
+  simp [toCube, foldl_cons, mem_vars, SetLike.ext_iff, Cube.mem_vars]
+  grind only
+
+@[simp]
+lemma models_toCube {n} {M : PartialModel n} : M.toCube.models = M.models := by
+  ext M'
+  simp [toCube, foldl_cons, mem_models]
+
+end PartialModel
+
+namespace Cube
+/-- Translate `δ` to a partial model. Returns `none` if `δ` is inconsistent. -/
+def toPartialModel {n} (δ : Cube n) : Option (PartialModel n) :=
+  δ.foldlM PartialModel.insert PartialModel.empty
+
+@[simp]
+lemma toPartialModel_eq_none_iff {n} {δ : Cube n} :
+    δ.toPartialModel = none ↔ δ.models = ∅ := by
+  suffices h1 : ∀ M, δ.foldlM PartialModel.insert M = none ↔ δ.models ∩ M.models = ∅ by
+    have := h1 PartialModel.empty
+    simp_all only [PartialModel.models_empty, Set.inter_univ, toPartialModel]
+  induction δ with
+  | nil =>
+    intro M
+    have := M.models_nonempty
+    simp_all only [Set.nonempty_iff_ne_empty, ne_eq, List.foldlM_nil, Option.pure_def, reduceCtorEq,
+      models_nil, Set.univ_inter]
+  | cons l δ' ih =>
+    intro M
+    simp only [List.foldlM_cons, Option.bind_eq_bind, Option.bind_eq_none_iff, models_cons, ih]
+    cases h1 : M.insert l with
+    | none =>
+      simp only [reduceCtorEq, IsEmpty.forall_iff, implies_true, Set.inter_assoc, true_iff]
+      rw [PartialModel.insert_eq_none_iff] at h1
+      grind [Literal.models_negate, PartialModel.subset_models_of_mem h1]
+    | some M' =>
+      have := M.models_insert h1
+      grind only [PartialModel.insert_eq_some_iff, Option.some.injEq]
+
+@[simp]
+lemma models_toPartialModel {n} {δ : Cube n} {M} :
+    δ.toPartialModel = some M → M.models = δ.models := by
+  suffices h1 :
+    ∀ M', (δ.foldlM PartialModel.insert M') = some M → M.models = δ.models ∩ M'.models by
+    intro h2
+    have := h1 PartialModel.empty h2
+    simp_all only [PartialModel.models_empty, Set.inter_univ]
+  induction δ generalizing M with
+  | nil =>
+    simp only [List.foldlM_nil, Option.pure_def, Option.some.injEq, models_nil, Set.univ_inter,
+      forall_eq]
+  | cons l δ' ih =>
+    simp_all only [List.foldlM_cons, Option.bind_eq_bind, models_cons, Option.bind_eq_some_iff]
+    rintro M'' ⟨M', h3, h4⟩
+    grind only [PartialModel.models_insert h3]
